proved that filter preserves well-formedness and promotability.
git-svn-id: https://webdav.seas.upenn.edu/svn/sol/vol@3969 eef5ea85-cc2e-0410-bd84-0fae1f012da8

src3.0/Transforms/filter.v
@@ -1,20 +1,10 @@
 Require Import vellvm.
 Require Import primitives.
 Require Import mem2reg.
-
-Lemma filter_ext: forall (A:Type) (f g:A->bool)
-  (Heq: forall a, f a = g a) (l0:list A), List.filter f l0 = List.filter g l0.
-Proof.
-  induction l0; intros; simpl; auto.
-    rewrite Heq. rewrite IHl0. auto.
-Qed.
-
-Lemma filter_true: forall (A:Type) (f:A->bool)
-  (Heq: forall a, f a = true) (l0:list A), l0 = List.filter f l0.
-Proof.
-  induction l0; intros; simpl; auto.
-    rewrite Heq. congruence.
-Qed.
+Require Import top_wfS.
+Require Import list_facts.
+Require Import palloca_props.
+Require Import trans_tactic.
 
 Section Filter.
 
@@ -36,34 +26,309 @@ Definition filter_fdef (f:fdef) : fdef :=
 let '(fdef_intro fh bs) := f in
 fdef_intro fh (List.map filter_block bs).
 
-Definition value_doesnt_use_removed (v:value): Prop :=
-forall instr, check instr = false -> used_in_value (getInsnLoc instr) v = false.
+Definition insnInFdef (instr:insn) (f:fdef) : Prop :=
+exists b, insnInFdefBlockB instr f b = true.
 
-Definition list_value_doesnt_use_removed (vl:list (sz * value)): Prop :=
+Definition id_isnt_removed f (id0:id): Prop :=
 forall instr, 
+  insnInFdef instr f ->
+  check instr = false -> id0 <> getInsnLoc instr.
+
+Definition value_doesnt_use_removed f (v:value): Prop :=
+forall instr, 
+  insnInFdef instr f ->
+  check instr = false -> used_in_value (getInsnLoc instr) v = false.
+
+Definition list_value_doesnt_use_removed f (vl:list (sz * value)): Prop :=
+forall instr, 
+  insnInFdef instr f ->
   check instr = false -> used_in_list_value (getInsnLoc instr) vl = false.
 
-Definition cmd_doesnt_use_removed (c:cmd): Prop :=
-forall instr, check instr = false -> used_in_cmd (getInsnLoc instr) c = false.
-
-Definition tmn_doesnt_use_removed (tmn:terminator): Prop :=
-forall instr, check instr = false -> used_in_tmn (getInsnLoc instr) tmn = false.
-
-Definition list_value_l_doesnt_use_removed (vl:list (value * l)): Prop :=
+Definition cmd_doesnt_use_removed f (c:cmd): Prop :=
 forall instr, 
+  insnInFdef instr f ->
+  check instr = false -> used_in_cmd (getInsnLoc instr) c = false.
+
+Definition tmn_doesnt_use_removed f (tmn:terminator): Prop :=
+forall instr, 
+  insnInFdef instr f ->
+  check instr = false -> used_in_tmn (getInsnLoc instr) tmn = false.
+
+Definition list_value_l_doesnt_use_removed f (vl:list (value * l)): Prop :=
+forall instr, 
+  insnInFdef instr f ->
   check instr = false -> used_in_list_value_l (getInsnLoc instr) vl = false.
 
-Definition phi_doesnt_use_removed (pn:phinode): Prop :=
-forall instr, check instr = false -> used_in_phi (getInsnLoc instr) pn = false.
+Definition phi_doesnt_use_removed f (pn:phinode): Prop :=
+forall instr, 
+  insnInFdef instr f ->
+  check instr = false -> used_in_phi (getInsnLoc instr) pn = false.
 
-Definition insn_doesnt_use_removed (inst:insn): Prop :=
-forall instr, check instr = false -> used_in_insn (getInsnLoc instr) inst = false.
+Definition insn_doesnt_use_removed f (inst:insn): Prop :=
+forall instr, 
+  insnInFdef instr f ->
+  check instr = false -> used_in_insn (getInsnLoc instr) inst = false.
 
-Definition block_doesnt_use_removed (b:block): Prop :=
-forall instr, check instr = false -> used_in_block (getInsnLoc instr) b = false.
+Definition block_doesnt_use_removed f (b:block): Prop :=
+forall instr, 
+  insnInFdef instr f ->
+  check instr = false -> used_in_block (getInsnLoc instr) b = false.
 
 Definition fdef_doesnt_use_removed (f:fdef): Prop :=
-forall instr, check instr = false -> used_in_fdef (getInsnLoc instr) f = false.
+forall instr, 
+  insnInFdef instr f ->
+  check instr = false -> 
+  used_in_fdef (getInsnLoc instr) f = false.
+
+Lemma id_isnt_removed__check: forall f instr
+  (Hlk: insnInFdef instr f)
+  (Hisnt: id_isnt_removed f (getInsnLoc instr)), check instr = true.
+Proof.
+  unfold id_isnt_removed.
+  intros.
+  remember (check instr) as R.
+  destruct R; auto.
+  symmetry in HeqR.
+  apply Hisnt in HeqR; auto.
+Qed.
+
+Lemma insn_doesnt_use_removed__id_isnt_removed: forall f (instr : insn)
+  (Hnouse : insn_doesnt_use_removed f instr),
+  Forall (id_isnt_removed f) (getInsnOperands instr).
+Proof.
+  intros.
+  apply Forall_forall.
+  intros.
+  intros insn Hlk Hck.
+  apply Hnouse in Hck; auto. subst.
+  apply noused_getInsnOperands in Hck.
+  intro EQ. subst. auto.
+Qed.
+
+Lemma list_value_l_doesnt_use_removed_cons_inv: forall f v0 l0 
+  (vl:list (value * l))
+  (Hnouse: list_value_l_doesnt_use_removed f ((v0,l0)::vl)),
+  value_doesnt_use_removed f v0 /\ list_value_l_doesnt_use_removed f vl.
+Proof.
+  intros.
+  split;
+    intros insn Hlk Hck; 
+    apply Hnouse in Hck; auto; simpl in Hck;
+    binvf Hck as J1 J2; auto.
+Qed.
+
+Lemma value_doesnt_use_removed__id_isnt_removed: forall f (vid : id)
+  (Hnouse : value_doesnt_use_removed f (value_id vid)),
+  id_isnt_removed f vid.
+Proof.
+  intros.
+  intros insn Hlk Hck.
+  apply Hnouse in Hck; auto.
+  intro EQ. subst. 
+  simpl in *. destruct_dec.
+Qed.
+
+Lemma insn_doesnt_use_removed__op_doesnt_use_removed : forall f instr v
+  (H2 : insn_doesnt_use_removed f instr)
+  (Hin : valueInInsnOperands v instr),
+  value_doesnt_use_removed f v.
+Proof.
+  intros.
+  intros insn Hlkup Hck.
+  apply H2 in Hck; auto.
+  apply noused_getInsnOperands in Hck.
+  destruct v; simpl; auto.
+  destruct_dec.
+    apply valueInInsnOperands__InOps in Hin. 
+    congruence.
+Qed.
+
+Lemma gep_doesnt_use_removed__idxs_dont_use_removed: forall 
+  (sz_value_list : list (sz * value)) (id5 : id) (inbounds5 : inbounds)
+  (typ5 : typ) (value_5 : value) (typ' : typ) f
+  (Hnouse : insn_doesnt_use_removed f
+              (insn_cmd
+                (insn_gep id5 inbounds5 typ5 value_5 sz_value_list typ')))
+  (v0 : value)
+  (Hin0 : In v0
+           (List.map
+              (fun pat_ : sz * value => let (_, value_) := pat_ in value_)
+              sz_value_list)),
+  value_doesnt_use_removed f v0.
+Proof.
+  intros.
+  eapply insn_doesnt_use_removed__op_doesnt_use_removed in Hnouse; eauto.
+  simpl. right.
+  apply InOps__valueInListValue'; auto.
+Qed.
+
+Lemma phi_doesnt_use_removed__incoming_dont_use_removed: forall 
+  (value_l_list : list (value * l)) (id5 : id) (typ5 : typ) f
+  (Hnouse : insn_doesnt_use_removed f
+             (insn_phinode (insn_phi id5 typ5 value_l_list)))
+  (v0 : value)
+  (Hin0 : In v0
+    (List.map (fun pat_ : value * l => let (value_, _) := pat_ in value_)
+       value_l_list)),
+  value_doesnt_use_removed f v0.
+Proof.
+  intros.
+  eapply insn_doesnt_use_removed__op_doesnt_use_removed in Hnouse; eauto.
+  simpl. 
+  apply InOps__in_list_prj1; auto.
+Qed.
+
+Lemma call_doesnt_use_removed__incoming_dont_use_removed: forall  
+  id5 noret5 clattrs5 typ1 varg5 value0 typ'_attributes'_value''_list f
+  (Hnouse : insn_doesnt_use_removed f
+             (insn_cmd
+                (insn_call id5 noret5 clattrs5 typ1 varg5 value0
+                   (List.map
+                      (fun pat_ : typ * attributes * value =>
+                       let (p, value_'') := pat_ in
+                       let (typ_', attributes_') := p in
+                       (typ_', attributes_', value_''))
+                      typ'_attributes'_value''_list))))
+  (value_'' : value) (typ_' : typ)
+  (H : In (value_'', typ_')
+        (List.map
+           (fun pat_ : typ * attributes * value =>
+            let (p, value_'') := pat_ in
+            let (typ_', _) := p in (value_'', typ_'))
+           typ'_attributes'_value''_list)),
+  value_doesnt_use_removed f value_''.
+Proof.
+  intros.
+  eapply insn_doesnt_use_removed__op_doesnt_use_removed in Hnouse; eauto.
+  simpl. right.
+  clear - H.
+  unfold valueInParams. 
+  induction typ'_attributes'_value''_list as [|[[]]]; simpl in *; auto.
+    destruct_let. 
+    simpl. 
+    destruct H as [H | H]; auto.
+    inv H. auto.
+Qed.
+
+Lemma block_doesnt_use_removed_inv: forall f l0 ps0 cs0 tmn0
+  (H: block_doesnt_use_removed f (block_intro l0 ps0 cs0 tmn0)),
+  insn_doesnt_use_removed f (insn_terminator tmn0) /\
+  Forall (phi_doesnt_use_removed f) ps0 /\
+  Forall (cmd_doesnt_use_removed f) cs0.
+Proof.
+  intros.
+  split.
+    intros instr Hlkp Hck.
+    apply H in Hck; auto.
+    binvf Hck as J1 J2.
+    binvf J1 as J3 J4.
+    auto.
+  split.
+    apply Forall_forall.
+    intros.
+    intros instr Hlkp Hck.
+    apply H in Hck; auto.
+    binvf Hck as J1 J2.
+    binvf J1 as J3 J4.
+    eapply fold_left_or_false_elim in J3; eauto.
+
+    apply Forall_forall.
+    intros.
+    intros instr Hlkp Hck.
+    apply H in Hck; auto.
+    binvf Hck as J1 J2.
+    binvf J1 as J3 J4.
+    eapply fold_left_or_false_elim in J4; eauto.
+Qed.
+
+Lemma fdef_doesnt_use_removed_inv: forall fh bs
+  (Hnouse : fdef_doesnt_use_removed (fdef_intro fh bs)),
+  List.Forall (block_doesnt_use_removed (fdef_intro fh bs)) bs.
+Proof.
+  intros.
+  apply Forall_forall.
+  intros.
+  intros instr Hlkup Hck.
+  apply Hnouse in Hck; auto.
+  simpl in Hck.
+  eapply fold_left_or_false_elim; eauto.
+Qed.
+
+Hint Resolve sl_nil sublist_refl.
+
+Lemma filter_block__blockLocs__sublist :
+  forall (bs : blocks),
+    sublist (getBlocksLocs (List.map filter_block bs))
+    (getBlocksLocs bs).
+Proof.
+  intros bs. induction bs as [|[lab phis cmds tmn] bs]. apply sl_nil.
+  simpl. repeat apply sublist_app; trivial; clear IHbs.
+  apply sublist_map. apply filter_sublist.
+  induction cmds as [|cmd cmds]. apply sl_nil.
+  simpl. 
+  destruct_if; simpl; try solve [apply sl_cons_r; auto | apply sl_cons; auto].
+Qed.
+
+Lemma filter_block__uniqBlocks :
+  forall (bs : blocks),
+    uniqBlocks bs -> uniqBlocks (List.map filter_block bs).
+Proof.
+  intros bs H.
+  split; [destruct H as [H _] | destruct H as [_ H]];
+    apply (NoDup_sublist _ _ _ H); clear H;
+      [|apply filter_block__blockLocs__sublist].
+  induction bs as [|[lab phis cmds tmn] bs]; simpl;
+    [apply sl_nil|apply sl_cons]; trivial.
+Qed.
+
+Lemma filter_fdef__uniqFdef :
+  forall (f : fdef),
+    uniqFdef f -> uniqFdef (filter_fdef f).
+Proof.
+  intros f H.
+  destruct f as [[att rtyp idf fas fvas] bs].
+  destruct H as [Hbsuniq HNoDup].
+  simpl. split. apply filter_block__uniqBlocks. trivial.
+  apply NoDup_split' in HNoDup. destruct HNoDup as [Hfas [Hbs Hin]].
+  apply NoDup_app. trivial.
+    apply NoDup_sublist with (getBlocksLocs bs). trivial.
+    apply filter_block__blockLocs__sublist.
+
+    intros id' H1 H2. clear Hbsuniq. apply (Hin id' H1).
+    clear H1. generalize id' H2. clear id' H2.
+    apply sublist_In. apply filter_block__blockLocs__sublist.
+Qed.
+
+Lemma filter_block__getBlockLabel: forall b,
+  getBlockLabel b = getBlockLabel (filter_block b).
+Proof.
+  destruct b as [l0 ? ? ?]; simpl; auto.
+Qed.
+
+Lemma filter_block__tmn_match: forall b, 
+  terminator_match (getBlockTmn b) (getBlockTmn (filter_block b)).
+Proof. 
+  destruct b as [l0 ? ? t0]; simpl. 
+  destruct t0; simpl; auto.
+Qed.
+
+Lemma filter_fdef_spec2: forall fh bs, 
+  filter_fdef (fdef_intro fh bs) = fdef_intro fh (List.map filter_block bs).
+Proof. simpl. auto. Qed.
+
+Lemma filter_fheader: forall f,
+  fheaderOfFdef f = fheaderOfFdef (filter_fdef f).
+Proof.
+  destruct f; auto.
+Qed.
+
+Definition Filter := mkPass 
+(filter_block)
+(filter_fdef)
+(filter_fdef_spec2)
+(filter_block__getBlockLabel)
+(filter_block__tmn_match)
+.
 
 End Filter.
 
@@ -116,7 +381,7 @@ Lemma fdef_doesnt_use_dead_insn: forall f
   fdef_doesnt_use_removed undead_insn f.
 Proof.
   intros.
-  intros instr Hcheck.
+  intros instr Hlkup Hcheck.
   apply undead_insn_false_inv in Hcheck. subst. auto.
 Qed.
 
@@ -131,7 +396,36 @@ end.
 Lemma fdef_doesnt_use_store: forall S M f (HwfF: wf_fdef S M f)
   (HuniqF: uniqFdef f),
   fdef_doesnt_use_removed isnt_store f.
-Admitted.
+Proof.
+  intros.
+  intros instr Hlkup Hck.
+  destruct Hlkup as [b Hlkup].
+  destruct instr as [|[]|]; inv Hck.
+  simpl.
+  remember (used_in_fdef id5 f) as R.
+  destruct R; auto.
+  symmetry in HeqR.
+  apply used_in_fdef_elim in HeqR.
+  destruct HeqR as [instr [b' [Hin Huse]]].
+  eapply wf_fdef__wf_insn in Hin; eauto 1.
+  apply wf_insn__wf_value with (v:=value_id id5) in Hin; auto.
+    destruct Hin as [t Hin].
+    inv Hin.
+    apply lookupTypViaIDFromFdef_elim in H4; auto.
+    destruct H4 as [[attr0 H4] | [b'' [instr' [H1 [H2 H3]]]]]; subst.
+      apply getArgsOfFdef__getArgsIDsOfFdef in H4.
+      contradict H4.
+      apply getInsnLoc__notin__getArgsIDs'' in Hlkup; auto.
+
+      apply IngetInsnsLocs__lookupInsnViaIDFromFdef in H1; auto.
+      apply IngetInsnsLocs__lookupInsnViaIDFromFdef in Hlkup; auto.
+      simpl in *.
+      rewrite H1 in Hlkup. 
+      inversion Hlkup. rewrite H3 in H2. simpl in H2.
+      clear - H0 H2. inv H2.
+      inv H0. inv H4.
+    apply used_in_insn__valueInInsnOperands; auto.
+Qed.
 
 Section ElimDeadStIsAFilter.
 
@@ -179,29 +473,1062 @@ Lemma fdef_doesnt_use_dead_store: forall S M f (HwfF: wf_fdef S M f)
 Proof.
   intros.
   apply fdef_doesnt_use_store in HwfF; auto.
-  intros instr Hcheck.
+  intros instr Hlk Hcheck.
   apply HwfF; auto.
   destruct instr as [ | [] | ]; auto.
 Qed.
 
 End ElimDeadStIsAFilter.
 
+Ltac fold_filter_tac :=
+repeat match goal with
+| |- context [filter_fdef ?chk ?f] =>
+  replace (filter_fdef chk f) with (ftrans (Filter chk) f); auto
+| |- context [filter_block ?chk ?b] =>
+  replace (filter_block chk b) with (btrans (Filter chk) b); auto
+| |- context [filter_fdef ?chk] =>
+  replace (filter_fdef chk) with (ftrans (Filter chk)); auto
+| |- context [filter_block ?chk] =>
+  replace (filter_block chk) with (btrans (Filter chk)); auto
+end.
+
 Lemma filter_successors : forall f check,
   successors f = successors (filter_fdef check f).
-Admitted.
+Proof.
+  intros.
+  fold_filter_tac.
+  apply TransCFG.pres_successors.
+Qed.
 
 Lemma filter_reachablity_analysis : forall f check,
   reachablity_analysis f = reachablity_analysis (filter_fdef check f).
-Admitted.
+Proof.
+  intros.
+  fold_filter_tac.
+  apply TransCFG.pres_reachablity_analysis.
+Qed.
+
+Section WellFormednessBasic.
+
+Variable check: insn -> bool.
+
+Lemma filter_InPhiNodesB : forall p 
+  (Hck: check (insn_phinode p) = true) ps
+  (Hin: InPhiNodesB p ps = true),
+  InPhiNodesB p (filter_phinodes check ps) = true.
+Proof.
+  induction ps; simpl; intros.
+    congruence.
+
+    binvt Hin as Hin Hin.
+      uniq_result. 
+      fill_ctxhole. 
+      solve_in_list.
+
+      destruct_if;
+        try solve [auto | apply orb_true_iff; right; auto].
+Qed.
+
+Hint Resolve filter_InPhiNodesB: ssa_filter.
+
+Lemma filter_phinodeInBlockB : forall p b
+  (Heq : check (insn_phinode p) = true)
+  (Hin : phinodeInBlockB p b = true),
+  phinodeInBlockB p (filter_block check b) = true.
+Proof.
+  destruct b. simpl. intro. auto with ssa_filter.
+Qed.
+
+Hint Resolve filter_phinodeInBlockB: ssa_filter.
+
+Lemma filter_InCmdsB : forall c 
+  (Hck: check (insn_cmd c) = true) cs
+  (Hin: InCmdsB c cs = true),
+  InCmdsB c (filter_cmds check cs) = true.
+Proof.
+  induction cs; simpl; intros; auto.
+    binvt Hin as Hin Hin.
+      uniq_result. 
+      fill_ctxhole. 
+      solve_in_list.
+
+      destruct_if;
+        try solve [auto | apply orb_true_iff; right; auto].
+Qed.
+
+Hint Resolve filter_InCmdsB: ssa_filter.
+
+Lemma filter_cmdInBlockB : forall c b
+  (Hck: check (insn_cmd c) = true)
+  (Hin : cmdInBlockB c b = true),
+  cmdInBlockB c (filter_block check b) = true.
+Proof.
+  destruct b. simpl. intro. auto with ssa_filter.
+Qed.
+
+Hint Resolve filter_cmdInBlockB: ssa_filter.
+
+Lemma filter_terminatorInBlockB : forall t b
+  (Hin : terminatorInBlockB t b = true),
+  terminatorInBlockB t (filter_block check b) = true.
+Proof.
+  destruct b. simpl. intro.
+  uniq_result. solve_refl.
+Qed.
+
+Hint Resolve filter_terminatorInBlockB: ssa_filter.
+
+Lemma filter_insnInFdefBlockB : forall f b instr
+  (Hneq : check instr = true \/ is_terminator instr = true)
+  (Hin : insnInFdefBlockB instr f b = true),
+  insnInFdefBlockB instr (filter_fdef check f) (filter_block check b) = true.
+Proof.
+  unfold insnInFdefBlockB.
+  intros.
+  destruct instr; simpl in *;
+    bdestruct Hin as J1 J2;
+    apply (@TransCFG.pres_blockInFdefB (Filter check)) in J2; auto;
+    simpl in J2;
+    match goal with
+    | H : _ \/ false = true |- _ => destruct H as [H | H]; try congruence
+    | _ => idtac
+    end;
+    bsplit; auto with ssa_filter.
+Qed.
+
+Hint Resolve filter_insnInFdefBlockB: ssa_filter.
+
+Lemma filter_In_getPhiNodesIDs1 : forall f id5
+  (Hck: id_isnt_removed check f id5) ps 
+  (Hbd: forall p, In p ps -> insnInFdef (insn_phinode p) f)
+  (Hin: In id5 (getPhiNodesIDs ps)),
+  In id5 (getPhiNodesIDs (filter_phinodes check ps)).
+Proof.
+  induction ps; simpl; intros. auto.
+    destruct Hin as [Hin | Hin]; subst.
+      erewrite id_isnt_removed__check; simpl; eauto.
+      destruct_if; simpl; auto.
+Qed.
+
+Lemma filter_In_getPhiNodesIDs2 : forall f id5 
+  (Hck: id_isnt_removed check f id5) ps
+  (Hbd: forall p, In p ps -> insnInFdef (insn_phinode p) f)
+  (Hin: In id5 (getPhiNodesIDs (filter_phinodes check ps))),
+  In id5 (getPhiNodesIDs ps).
+Proof.
+  induction ps; simpl; intros; auto.
+    destruct_if; auto.
+Qed.
+
+Lemma filter_In_getCmdsIDs1 : forall f id5
+  (Hck: id_isnt_removed check f id5) cs
+  (Hbd: forall c, In c cs -> insnInFdef (insn_cmd c) f)
+  (Hin: In id5 (getCmdsIDs cs)),
+  In id5 (getCmdsIDs (filter_cmds check cs)).
+Proof.
+  induction cs as [|c]; simpl; intros. auto.
+    remember (getCmdID c) as R.
+    destruct R. 
+      symmetry_ctx.
+      assert (J:=HeqR).
+      apply getCmdID__getCmdLoc in HeqR. subst.
+      simpl in Hin.
+      destruct Hin as [Hin | Hin]; subst.
+        erewrite id_isnt_removed__check; simpl; eauto.
+        fill_ctxhole. simpl. auto.
+
+        destruct_if; simpl; auto.
+        fill_ctxhole. simpl. auto.
+      destruct_if; simpl; auto.
+      fill_ctxhole. simpl. auto.
+Qed.
+
+Lemma filter_In_getCmdsIDs2 : forall f id5
+  (Hck: id_isnt_removed check f id5) cs
+  (Hbd: forall c, In c cs -> insnInFdef (insn_cmd c) f)
+  (Hin: In id5 (getCmdsIDs (filter_cmds check cs))),
+  In id5 (getCmdsIDs cs).
+Proof.
+  induction cs as [|c]; simpl; intros. auto.
+    destruct_if; simpl in *; auto.
+    destruct (getCmdID c); auto.
+    destruct_in Hin; simpl; auto.
+
+    destruct (getCmdID c); simpl; auto.
+Qed.
+
+Lemma blockInFdefB__phiInFdef: forall l5 ps cs tmn f
+  (Hbd: blockInFdefB (block_intro l5 ps cs tmn) f = true),
+  forall p, In p ps -> insnInFdef (insn_phinode p) f.
+Proof.
+  intros.
+  exists (block_intro l5 ps cs tmn).
+  bsplit; auto.
+    simpl. solve_in_list.
+Qed.
+
+Lemma blockInFdefB__cmdInFdef: forall l5 ps cs tmn f
+  (Hbd: blockInFdefB (block_intro l5 ps cs tmn) f = true),
+  forall c, In c cs -> insnInFdef (insn_cmd c) f.
+Proof.
+  intros.
+  exists (block_intro l5 ps cs tmn).
+  bsplit; auto.
+    simpl. solve_in_list.
+Qed.
+
+Hint Resolve filter_In_getPhiNodesIDs1 filter_In_getCmdsIDs1
+             filter_In_getPhiNodesIDs2 filter_In_getCmdsIDs2 
+             blockInFdefB__phiInFdef blockInFdefB__cmdInFdef: ssa_filter.
+
+Lemma filter_lookupBlockViaIDFromBlocks : forall f id5 bs b
+  (Hck: id_isnt_removed check f id5) 
+  (Hbd: forall b, In b bs -> blockInFdefB b f = true)
+  (Hin: lookupBlockViaIDFromBlocks bs id5 = ret b),
+  lookupBlockViaIDFromBlocks (List.map (filter_block check) bs) id5 =
+    ret (filter_block check b).
+Proof.
+  induction bs as [|[l5 p c t5]]; simpl; intros.
+    congruence.
+
+    assert (blockInFdefB (block_intro l5 p c t5) f = true) as Hbd' by auto.
+    destruct_if;
+      destruct_if; try solve [
+        auto |
+        match goal with
+        | HeqR: left ?i0 = _, HeqR0: right ?n = _ |- _ =>
+          clear HeqR0 HeqR; contradict n;
+          apply in_or_app;
+          destruct_in i0; eauto with ssa_filter
+        end
+      ].
+Qed.
+
+Lemma blockInFdefB__blocksInFdefB: forall fh bs b, 
+  In b bs -> blockInFdefB b (fdef_intro fh bs) = true.
+Proof. simpl. intros. solve_in_list. Qed.
+
+Hint Resolve filter_lookupBlockViaIDFromBlocks 
+             blockInFdefB__blocksInFdefB: ssa_filter.
+
+Lemma filter_lookupBlockViaIDFromFdef : forall f id5 b
+  (Hck: id_isnt_removed check f id5)
+  (Hin: lookupBlockViaIDFromFdef f id5 = ret b),
+  lookupBlockViaIDFromFdef (filter_fdef check f) id5 = 
+    ret (filter_block check b).
+Proof.
+  destruct f. simpl; intros. eauto with ssa_filter.
+Qed.
+
+Hint Resolve filter_lookupBlockViaIDFromFdef: ssa_filter.
+
+Hint Resolve not_id_dec__neq : ssa_filter.
+
+Lemma filter_phinodes_neq : forall p1 ps2 ps1
+  (Hck: check (insn_phinode p1) = true), 
+  exists ps0, exists ps3,
+    filter_phinodes check (ps1 ++ p1 :: ps2) = ps0 ++ p1 :: ps3 /\
+    filter_phinodes check ps1 = ps0 /\
+    filter_phinodes check ps2 = ps3.
+Proof.
+  induction ps1 as [|a]; intros; simpl.
+    fill_ctxhole. 
+    exists nil. exists (filter_phinodes check ps2). auto.
+
+    destruct_if; auto.
+    apply IHps1 in Hck. destruct Hck as [ps0 [ps3 [H [J1 J2]]]].
+    exists (a::ps0). exists ps3. rewrite H. rewrite J1. rewrite J2. auto.
+Qed.
+
+Lemma filter_cmds_neq : forall cs2 c1 cs1
+  (Hck: check (insn_cmd c1) = true), 
+   exists cs0 : list cmd,
+     exists cs4 : list cmd,
+       filter_cmds check (cs1 ++ c1 :: cs2) = cs0 ++ c1 :: cs4 /\
+       filter_cmds check cs1 = cs0 /\
+       filter_cmds check cs2 = cs4.
+Proof.
+  induction cs1 as [|a]; intros; simpl.
+    fill_ctxhole. 
+    exists nil. exists (filter_cmds check cs2). auto.
+
+    destruct_if; auto.
+    apply IHcs1 in Hck. destruct Hck as [cs0 [cs3 [H [J1 J2]]]].
+    exists (a::cs0). exists cs3. rewrite H. rewrite J1. rewrite J2. auto.
+Qed.
+
+Lemma filter_phinodes_neq_inv : forall ps p1 ps3 ps0
+  (Hck: check (insn_phinode p1) = true)
+  (Heq: filter_phinodes check ps  = ps0 ++ p1 :: ps3),
+  exists ps1, exists ps2,
+    ps = ps1 ++ p1 :: ps2 /\
+    filter_phinodes check ps1 = ps0 /\
+    filter_phinodes check ps2 = ps3.
+Proof.
+  induction ps as [|a]; simpl; intros.
+    solve_in_list'.
+
+    destruct_if.
+      destruct ps0; inv H0.
+        exists nil. exists ps. auto.
+
+        apply IHps in H2; auto.
+        destruct H2 as [ps1 [ps2 [H3 [J1 J2]]]]; subst.
+        exists (p::ps1). exists ps2. simpl.
+        destruct_if.
+          congruence.
+
+      apply IHps in H0; auto.
+      destruct H0 as [ps1 [ps2 [H0 [J1 J2]]]]; subst.
+      exists (a::ps1). exists ps2. simpl.
+      destruct_if.
+        congruence.
+Qed.
+
+Lemma filter_cmds_neq_inv : forall cs c1 cs3 cs0
+  (Hck: check (insn_cmd c1) = true)
+  (Heq: filter_cmds check cs  = cs0 ++ c1 :: cs3),
+  exists cs1, exists cs2,
+    cs = cs1 ++ c1 :: cs2 /\
+    filter_cmds check cs1 = cs0 /\
+    filter_cmds check cs2 = cs3.
+Proof.
+  induction cs as [|a]; simpl; intros.
+    solve_in_list'.
+
+    destruct_if.
+      destruct cs0; inv H0.
+        exists nil. exists cs. auto.
+
+        apply IHcs in H2; auto.
+        destruct H2 as [cs1 [cs2 [H3 [J1 J2]]]]; subst.
+        exists (c::cs1). exists cs2. simpl.
+        destruct_if.
+          congruence.
+
+      apply IHcs in H0; auto.
+      destruct H0 as [cs1 [cs2 [H0 [J1 J2]]]]; subst.
+      exists (a::cs1). exists cs2. simpl.
+      destruct_if.
+        congruence.
+Qed.
+
+Ltac unfold_getInsnLoc :=
+repeat match goal with
+| H: context [getPhiNodeID ?p] |- _ => 
+     replace (getPhiNodeID p) with (getInsnLoc (insn_phinode p)) in H; auto
+| H: context [getCmdLoc ?c] |- _ => 
+     replace (getCmdLoc c) with (getInsnLoc (insn_cmd c)) in H; auto
+| H: context [getTerminatorID ?t] |- _ => 
+     replace (getTerminatorID t) with (getInsnLoc (insn_terminator t)) in H; auto
+end.
+
+Ltac find_insnInFdef_tac :=
+match goal with
+| H: blockInFdefB ?b _ = true |- _ =>
+  exists b; simpl; bsplit; auto; solve_in_list
+end.
+
+Lemma filter_insnDominates_tmn : forall f i0 instr b
+  (Hnodup: NoDup (getBlockLocs b))
+  (Heq1: is_terminator instr = true)
+  (Heq2: id_isnt_removed check f i0)
+  (HiInF: insnInFdefBlockB instr f b = true),
+  insnDominates i0 instr b ->
+  insnDominates i0 instr (filter_block check b).
+Proof.
+ intros f i0 instr b Hnodup Hneq1 Hneq2 HiInF. 
+ apply destruct_insnInFdefBlockB in HiInF.
+ destruct HiInF as [HiInB HbInF].
+ destruct b as [l0 ps cs tmn]. 
+ destruct instr as [|c0|]; tinv Hneq1; simpl; intro J; auto.
+ simpl in HiInB. uniq_result.
+   destruct J as [[[cs1 [c1 [cs2 [J1 J2]]]] | [ps1 [p1 [ps2 [J1 J2]]]]] Heq];
+     subst; split; auto.
+     left.
+     assert (J2':=J2).
+     apply getCmdLoc_getCmdID in J2. subst.
+     unfold_getInsnLoc.
+     apply id_isnt_removed__check in Hneq2; try find_insnInFdef_tac.
+     apply filter_cmds_neq with (cs1:=cs1)(cs2:=cs2) in Hneq2; eauto.
+     destruct Hneq2 as [cs0 [cs3' [Heq2 [J5 J6]]]].
+     rewrite Heq2. exists cs0. exists c1. exists cs3'. split; auto.
+
+     right.
+     unfold_getInsnLoc.
+     apply id_isnt_removed__check in Hneq2; try find_insnInFdef_tac.
+     apply filter_phinodes_neq with (ps1:=ps1)(ps2:=ps2) in Hneq2; eauto.
+     destruct Hneq2 as [ps0 [ps3 [Heq2 [J5 J6]]]].
+     rewrite Heq2. eauto.
+Qed.
+
+Lemma filter_insnDominates : forall f i0 instr b
+  (Hnodup: NoDup (getBlockLocs b))
+  (Heq1: check instr = true \/ is_terminator instr = true)
+  (Heq2: id_isnt_removed check f i0)
+  (HiInF: insnInFdefBlockB instr f b = true),
+  (insnDominates i0 instr b ->
+  insnDominates i0 instr (filter_block check b)).
+Proof.
+ intros f i0 instr b Hnodup Hneq1 Hneq2 HiInF. 
+ remember (is_terminator instr) as R.
+ destruct R; eauto using filter_insnDominates_tmn.
+ destruct Hneq1 as [Hneq1 | Hneq1]; try congruence.
+ apply destruct_insnInFdefBlockB in HiInF.
+ destruct HiInF as [HiInB HbInF].
+ destruct b as [l0 ps cs tmn]. simpl.
+ destruct instr as [|c0|]; tinv HeqR; simpl; intro J; auto.
+   destruct J as [[ps1 [p1 [ps2 [J1 J2]]]] | [cs1 [c1 [cs2 [cs3 [J1 J2]]]]]];
+     subst.
+     left.
+     unfold_getInsnLoc.
+     apply id_isnt_removed__check in Hneq2; try find_insnInFdef_tac.
+     apply filter_phinodes_neq with (ps1:=ps1)(ps2:=ps2) in Hneq2; eauto.
+     destruct Hneq2 as [ps0 [ps3 [Heq2 [J5 J6]]]].
+     rewrite Heq2. eauto.
+
+     right. simpl in Hneq1.
+     assert (J2':=J2).
+     apply getCmdLoc_getCmdID in J2. subst.
+     unfold_getInsnLoc.
+     apply id_isnt_removed__check in Hneq2; try find_insnInFdef_tac.
+     apply filter_cmds_neq with (cs1:=cs1)(cs2:=cs2 ++ c0 :: cs3) in Hneq2; eauto.
+     destruct Hneq2 as [cs0 [cs3' [Heq2 [J5 J6]]]].
+     rewrite Heq2. exists cs0. exists c1. rewrite <- J6.
+     apply filter_cmds_neq with (cs1:=cs2)(cs2:=cs3) in Hneq1; eauto.
+     destruct Hneq1 as [cs4 [cs5 [Hneq1 [J7 J8]]]].
+     rewrite Hneq1. exists cs4. exists cs5. split; auto.
+Qed.
+
+Lemma filter_wf_operand : forall instr f b i0
+  (Huniq : NoDup (getBlockLocs b))
+  (H1 : wf_operand f b instr i0)
+  (Hneq : check instr = true \/ is_terminator instr = true)
+  (Heq2: id_isnt_removed check f i0),
+  wf_operand (filter_fdef check f) (filter_block check b) instr i0.
+Proof.
+  intros.
+  inv H1.
+  eapply wf_operand_intro; try solve [eauto with ssa_filter].
+    fold_filter_tac.
+    rewrite <- TransCFG.pres_isReachableFromEntry.
+    rewrite <- TransCFG.pres_getArgsIDsOfFdef.
+    match goal with
+    | H4: (_ \/ _ ) \/ _ |- _ => 
+        destruct H4 as [[[b' [H5 H4]] | H4] | H4]; auto
+    end.
+    left. left.
+    exists (btrans (Filter check) b').
+      rewrite <- TransCFG.pres_blockStrictDominates.
+      simpl.
+      split; auto with ssa_filter.
+      match goal with
+      | H4: _ \/ blockStrictDominates _ _ _ |- _ =>
+        destruct H4 as [H4 | H4]; auto
+      end.
+        left.
+        eapply filter_insnDominates; eauto.
+Qed.
+
+Hint Resolve filter_wf_operand: ssa_filter.
+
+Lemma filter_wf_operand_list : forall instr f b 
+  (Huniq : NoDup (getBlockLocs b))
+  (Hneq : check instr = true \/ is_terminator instr = true) id_list0
+  (Hnotin : List.Forall (id_isnt_removed check f) id_list0)
+  (H2 : forall id_ : id,
+          In id_ (List.map (fun id_0 : id => id_0) id_list0) ->
+          wf_operand f b instr id_),
+  forall id_ : id,
+    In id_ (List.map (fun id_0 : id => id_0) id_list0) ->
+    wf_operand (filter_fdef check f) (filter_block check b)
+       instr id_.
+Proof.
+  induction 3; simpl; intros; auto.
+    tauto.
+  
+    destruct H0 as [H0 | H0]; subst; auto.
+      auto with ssa_filter.
+Qed.
+
+Hint Resolve filter_wf_operand_list: ssa_filter.
+
+Hint Resolve insn_doesnt_use_removed__id_isnt_removed: ssa_filter.
+
+Lemma filter_wf_insn_base : forall f b instr
+  (Huniq : NoDup (getBlockLocs b))
+  (Hneq : check instr = true \/ is_terminator instr = true)
+  (Hnouse : insn_doesnt_use_removed check f instr)
+  (HwfI: wf_insn_base f b instr),
+  wf_insn_base (filter_fdef check f) (filter_block check b) instr.
+Proof.
+  intros.
+  inv HwfI.
+  eapply filter_insnInFdefBlockB in H; eauto.
+  subst.
+  eapply wf_insn_base_intro; eauto with ssa_filter.
+Qed.
+
+Hint Constructors wf_phi_operands.
+
+Hint Resolve value_doesnt_use_removed__id_isnt_removed: ssa_filter.
+
+Lemma filter_wf_phi_operands : forall f b ty id' vls
+  (Hnouse : list_value_l_doesnt_use_removed check f vls)
+  (Hwf_pnops: wf_phi_operands f b id' ty vls),
+  wf_phi_operands (filter_fdef check f) (filter_block check b) id' ty vls.
+Proof.
+  intros.
+  induction Hwf_pnops; simpl in *; auto.
+    apply list_value_l_doesnt_use_removed_cons_inv in Hnouse.
+    destruct Hnouse as [J1 J2].
+    eapply wf_phi_operands_cons_vid; eauto.
+      fold_filter_tac.
+      eapply TransCFG.pres_lookupBlockViaLabelFromFdef in H; eauto.
+
+      fold_filter_tac.
+      rewrite <- TransCFG.pres_getArgsIDsOfFdef; auto.
+      rewrite <- TransCFG.pres_isReachableFromEntry; auto.
+      destruct H0 as [[[vb [J1' J2']] | H0] | H0]; auto.
+      left. left.
+      exists (filter_block check vb).
+      eapply filter_lookupBlockViaIDFromFdef in J1'; eauto with ssa_filter.
+      fold_filter_tac.
+      rewrite <- TransCFG.pres_blockDominates; auto.
+Qed.
+
+Hint Resolve filter_wf_phi_operands: ssa_filter.
+
+Lemma filter_wf_phinode : forall f b PN (HwfPN: wf_phinode f b PN)
+  (Hnouse: phi_doesnt_use_removed check f PN),
+  wf_phinode (filter_fdef check f) (filter_block check b) PN.
+Proof.
+  intros. destruct PN as [id' vls].
+  unfold wf_phinode in *. simpl.
+  destruct HwfPN as [Hwf_pnops Hcl].
+  split; auto with ssa_filter.
+    fold_filter_tac.
+    apply TransCFG.pres_check_list_value_l; auto.
+Qed.
+
+Lemma filter_lookupTypViaIDFromPhiNodes : forall f id5
+  (Hneq: id_isnt_removed check f id5) ps
+  (Hbd: forall p, In p ps -> insnInFdef (insn_phinode p) f),
+  lookupTypViaIDFromPhiNodes ps id5 =
+    lookupTypViaIDFromPhiNodes (filter_phinodes check ps) id5.
+Proof.
+  induction ps as [|a]; simpl; intros; auto.
+    rewrite IHps; auto.
+    destruct a. simpl.
+    unfold lookupTypViaIDFromPhiNode in *.
+    destruct_if.
+      erewrite id_isnt_removed__check; eauto.
+      simpl.
+      unfold lookupTypViaIDFromPhiNode in *. simpl.
+      destruct_if.
+        congruence.
+
+      destruct_if.
+        simpl.
+        unfold lookupTypViaIDFromPhiNode in *. simpl in *.
+        destruct_if.
+          congruence.
+Qed.
+
+Lemma filter_lookupTypViaIDFromCmds : forall f id5 
+  (Hneq: id_isnt_removed check f id5) cs
+  (Hbd: forall c, In c cs -> insnInFdef (insn_cmd c) f),
+  lookupTypViaIDFromCmds cs id5 = lookupTypViaIDFromCmds (filter_cmds check cs) id5.
+Proof.
+  induction cs as [|a]; simpl; intros; auto.
+    rewrite IHcs; auto.
+    unfold lookupTypViaIDFromCmd in *.
+    assert (J:=getCmdTyp__total a).
+    remember (getCmdTyp a) as R.
+    destruct R; try congruence.
+    destruct_if. 
+      erewrite id_isnt_removed__check; eauto.
+      simpl.
+      unfold lookupTypViaIDFromCmd in *. simpl.
+      rewrite <- HeqR.
+      destruct_if.
+        congruence.
+
+      destruct_if.
+        simpl.
+        unfold lookupTypViaIDFromCmd in *. simpl in *.
+        rewrite <- HeqR.
+        destruct_if.
+          congruence.
+Qed.
+
+Lemma filter_lookupTypViaIDFromBlocks : forall f id5
+  (Hneq: id_isnt_removed check f id5) bs
+  (Hbd: forall b, In b bs -> blockInFdefB b f = true),
+  lookupTypViaIDFromBlocks bs id5 =
+    lookupTypViaIDFromBlocks (List.map (filter_block check) bs) id5.
+Proof.
+  induction bs as [|[l5 p c t5]]; simpl; intros; auto.
+    rewrite IHbs; auto.
+    assert (blockInFdefB (block_intro l5 p c t5) f = true) as Hbd' by auto.
+    erewrite <- filter_lookupTypViaIDFromPhiNodes; eauto with ssa_filter.
+    erewrite <- filter_lookupTypViaIDFromCmds; eauto with ssa_filter.
+Qed.
+
+Lemma filter_lookupTypViaIDFromFdef : forall f id5
+  (Hneq: id_isnt_removed check f id5),
+  lookupTypViaIDFromFdef f id5 = lookupTypViaIDFromFdef (filter_fdef check f) id5.
+Proof.
+  destruct f. simpl. intros. 
+  erewrite <- filter_lookupTypViaIDFromBlocks; eauto with ssa_filter.
+Qed.
+
+End WellFormednessBasic.
+
+Section WellFormedness.
+
+Variable (los:layouts) (nts:namedts) (Ps1 Ps2:products)
+         (M M':module) (f f':fdef) (check:insn -> bool).
+Hypothesis (HeqM: M = module_intro los nts (Ps1 ++ product_fdef f :: Ps2))
+           (HeqM': M' = module_intro los nts (Ps1 ++ product_fdef f' :: Ps2))
+           (HeqF': f' = filter_fdef check f).
+
+Lemma filter_wf_typ: forall t,
+  wf_typ [M] (los,nts) t -> wf_typ [M'] (los,nts) t.
+Proof.
+  subst.
+  eapply TopWFS.subst_fdef_preserves_single_wf_typ; 
+    eauto using filter_fheader.
+Qed.
+
+Lemma filter_wf_const: forall c t,
+  wf_const [M] (los,nts) c t -> wf_const [M'] (los,nts) c t.
+Proof.
+  subst.
+  eapply TopWFS.subst_fdef_preserves_single_wf_const;
+    eauto using filter_fheader.
+Qed.
+
+Lemma filter_blockInSystemModuleFdefB: forall b b'
+  (Heqb': b' = filter_block check b) 
+  (Hin: blockInSystemModuleFdefB b [M] M f),
+  blockInSystemModuleFdefB b' [M'] M' f'.
+Proof.
+  intros.
+  subst.
+  apply blockInSystemModuleFdef_inv in Hin.
+  destruct Hin as [J1 [J2 [J3 J4]]].
+  apply blockInSystemModuleFdef_intro.
+    fold_filter_tac.
+    apply TransCFG.pres_blockInFdefB; auto.
+
+    apply InProductsB_middle.
+
+    unfold moduleInSystem. simpl.
+    apply orb_true_intro.
+    left. solve_refl.
+Qed.
+
+Lemma filter_preserves_wf_fheader: forall fh,
+  wf_fheader [M] (los,nts) fh -> wf_fheader [M'] (los,nts) fh.
+Proof.
+  subst.
+  eapply TopWFS.subst_fdef_preserves_single_wf_fheader; 
+    eauto using filter_fheader.
+Qed.
+
+Hint Constructors wf_insn wf_value.
+
+Hint Resolve value_doesnt_use_removed__id_isnt_removed: ssa_filter.
+
+Lemma filter_wf_value : forall v t (Hwfv: wf_value [M] M f v t)
+  (Hnouse : value_doesnt_use_removed check f v),
+  wf_value [M'] M' f' v t.
+Proof.
+  intros.
+  assert (J1:=filter_wf_const).
+  assert (J3:=filter_wf_typ).
+  subst. 
+  inv Hwfv; try constructor; eauto.
+    rewrite <- filter_lookupTypViaIDFromFdef; auto with ssa_filter.
+Qed.
+
+Hint Resolve filter_wf_value : ssa_filter.
+
+Ltac filter_wf_cmd_tac :=
+match goal with
+| H2: wf_insn_base _ _ _ |- wf_insn_base _ _ _ =>
+   eapply filter_wf_insn_base in H2; eauto
+| _ => auto
+end.
+
+Lemma filter_wf_trunc : forall b b' 
+  (Huniq: NoDup (getBlockLocs b))
+  (Heqb': b' = filter_block check b) instr
+  (Hnr : check instr = true)
+  (Hnouse : insn_doesnt_use_removed check f instr)
+  (HwfI : wf_trunc [M] M f b instr),
+  wf_trunc [M'] M' f' b' instr.
+Proof.
+  intros.
+  assert (J2:=filter_wf_value).
+  assert (J1:=filter_wf_typ).
+  inv HwfI; uniq_result; try solve [
+    econstructor; try solve [filter_wf_cmd_tac]
+  ].
+Qed.
+
+Lemma filter_wf_ext : forall b b' 
+  (Huniq: NoDup (getBlockLocs b))
+  (Heqb': b' = filter_block check b) instr
+  (Hnr : check instr = true)
+  (Hnouse : insn_doesnt_use_removed check f instr)
+  (HwfI : wf_ext [M] M f b instr),
+  wf_ext [M'] M' f' b' instr.
+Proof.
+  intros.
+  assert (J2:=filter_wf_value).
+  assert (J1:=filter_wf_typ).
+  inv HwfI; uniq_result; try solve [
+    econstructor; try solve [filter_wf_cmd_tac]
+  ].
+Qed.
+
+Lemma filter_wf_cast : forall b b' 
+  (Huniq: NoDup (getBlockLocs b))
+  (Heqb': b' = filter_block check b) instr
+  (Hnr : check instr = true)
+  (Hnouse : insn_doesnt_use_removed check f instr)
+  (HwfI : wf_cast [M] M f b instr),
+  wf_cast [M'] M' f' b' instr.
+Proof.
+  intros.
+  assert (J2:=filter_wf_value).
+  assert (J1:=filter_wf_typ).
+  inv HwfI; uniq_result; try solve [
+    econstructor; try solve [filter_wf_cmd_tac]
+  ].
+Qed.
+
+Lemma filter_wf_value_list : forall t vs
+  (Hnouse : List.Forall (value_doesnt_use_removed check f) vs)
+  (H :forall value_ : value, In value_ vs -> wf_value [M] M f value_ t),
+  forall (value_ : value) (Hin: In value_ vs), wf_value [M'] M' f' value_ t.
+Proof.
+  assert (J:=filter_wf_value).
+  induction 1; simpl; intros.
+    tauto.
+    destruct Hin as [Hin | Hin]; subst; auto.
+Qed.
+
+Hint Resolve filter_wf_value_list: ssa_filter.
+
+Lemma filter_wf_insn : forall b instr (HwfI: wf_insn [M] M f b instr)
+  (Huniq : NoDup (getBlockLocs b)) 
+  (Hnouse : insn_doesnt_use_removed check f instr)
+  (Hnr : check instr = true \/ is_terminator instr = true) 
+  b' (Heqb': b' = filter_block check b),
+  wf_insn [M'] M' f' b' instr.
+Proof.
+  intros.
+  assert (J1:=filter_wf_value_list).
+  assert (J2:=filter_wf_value).
+  assert (J3:=filter_wf_typ).
+  assert (J5:=@filter_wf_trunc b b' Huniq Heqb' instr).
+  assert (J6:=@filter_wf_ext b b' Huniq Heqb' instr).
+  assert (J7:=@filter_wf_cast b b' Huniq Heqb' instr).
+  assert (J8:=filter_wf_const).
+
+Ltac filter_wf_insn_pre_tac :=
+repeat match goal with
+| H1 : context [Function.getDefReturnType f] |- _ =>
+  rewrite <- 
+    (@TransCFG.pres_getDefReturnType (Filter check)) in H1
+| |- context [Function.getDefReturnType f] =>
+  rewrite <- 
+    (@TransCFG.pres_getDefReturnType (Filter check)); auto
+| H1 : lookupBlockViaLabelFromFdef f _ = ret _ |- _ =>
+  apply (@TransCFG.pres_lookupBlockViaLabelFromFdef 
+           (Filter check)) in H1
+end.
+
+Ltac remove_is_tmn_tac :=
+  match goal with
+  | H : _ \/ is_terminator _ = true |- _ => 
+      simpl in H; destruct H as [H | H]; try congruence
+  end.
+
+Ltac filter_wf_insn_post_tac :=
+match goal with
+| |- wf_trunc _ _ _ _ _ => remove_is_tmn_tac
+| |- wf_ext _ _ _ _ _ => remove_is_tmn_tac
+| |- wf_cast _ _ _ _ _ => remove_is_tmn_tac
+| |- _ => idtac
+end;
+match goal with
+| H1 : insnInFdefBlockB _ _ _ = true |- insnInFdefBlockB _ _ _ = true =>
+  eapply filter_insnInFdefBlockB in H1; eauto
+| H2: wf_insn_base _ _ _ |- wf_insn_base _ _ _ => 
+  eapply filter_wf_insn_base in H2; eauto
+| H2: wf_phinode _ _ _ |- wf_phinode _ _ _ => 
+   eapply filter_wf_phinode in H2; eauto
+| H2: insn_doesnt_use_removed _ _ _,
+  J2: forall _ _, _ -> _ -> wf_value _ _ _ _ _ |- wf_value _ _ _ _ _ =>
+   eapply J2; try solve [
+     eauto 2 |
+     eapply insn_doesnt_use_removed__op_doesnt_use_removed in H2; simpl; eauto
+   ]
+| H2: insn_doesnt_use_removed _ _ _,
+  J2: forall _ _, _ -> _ -> wf_value _ _ _ _ _
+  |- context [ In _ _ -> wf_value _ _ _ _ _ ] =>
+   intros;
+   eapply J2; try solve [
+     eauto 2 |
+     eapply gep_doesnt_use_removed__idxs_dont_use_removed in H2; simpl; eauto |
+     eapply phi_doesnt_use_removed__incoming_dont_use_removed in H2; simpl; eauto |
+     eapply call_doesnt_use_removed__incoming_dont_use_removed in H2; simpl; eauto
+   ]
+| _ => eauto with ssa_filter
+end.
+
+  inv HwfI; uniq_result; try solve [
+    filter_wf_insn_pre_tac;
+    econstructor; 
+    filter_wf_insn_post_tac
+  ].
+Qed.
+
+Hint Resolve filter_wf_insn : ssa_filter.
+
+Hint Constructors wf_phinodes.
+
+Lemma filter_wf_phinodes : forall b PNs (HwfPNs: wf_phinodes [M] M f b PNs)
+  (Hnouse : List.Forall (phi_doesnt_use_removed check f) PNs)
+  (Huniq : NoDup (getBlockLocs b)) b' (Heqb': b' = filter_block check b),
+  wf_phinodes [M'] M' f' b' (filter_phinodes check PNs).
+Proof.
+  assert (J:=filter_wf_insn).
+  subst.
+  induction 2; simpl in *; intros; auto.
+    inv HwfPNs.
+    destruct_if; eauto.
+Qed.
+
+Hint Constructors wf_cmds.
+
+Lemma filter_wf_cmds : forall b Cs (HwfCs: wf_cmds [M] M f b Cs)
+  (Hnouse : List.Forall (cmd_doesnt_use_removed check f) Cs)
+  (Huniq : NoDup (getBlockLocs b)) b' (Heqb': b' = filter_block check b),
+  wf_cmds [M'] M' f' b' (filter_cmds check Cs).
+Proof.
+  assert (J:=filter_wf_insn).
+  subst.
+  induction 2; simpl in *; intros; auto.
+    inv HwfCs.
+    destruct_if; eauto.
+Qed.
+
+Lemma filter_wf_block : forall b (HwfB : wf_block [M] M f b)
+  (Hnouse : block_doesnt_use_removed check f b)
+  (Huniq : NoDup (getBlockLocs b)) b' (Heqb': b' = filter_block check b),
+  wf_block [M'] M' f' b'.
+Proof.
+  intros.
+  inv_wf_block HwfB. subst b.
+  apply block_doesnt_use_removed_inv in Hnouse.
+  destruct Hnouse as [Hnouse1 [Hnouse2 Hnouse3]].
+  eapply filter_blockInSystemModuleFdefB in HBinSMF; eauto.
+  eapply filter_wf_cmds in Hwfcs; eauto.
+  eapply filter_wf_phinodes in Hwfps; eauto.
+  eapply filter_wf_insn in Hwfi; eauto 1; simpl; auto.
+    subst. apply wf_block_intro; eauto.
+Qed.
+
+Hint Resolve filter_wf_block : ssa_filter.
+
+Hint Constructors wf_blocks.
+
+Lemma filter_wf_blocks : forall bs (HwfBs : wf_blocks [M] M f bs)
+  (Hnouse : List.Forall (block_doesnt_use_removed check f) bs)
+  (Huniq : NoDup (getBlocksLocs bs)),
+  wf_blocks [M'] M' f' (List.map (filter_block check) bs).
+Proof.
+  induction 2; simpl; intros.
+    constructor.
+
+    simpl in Huniq.
+    split_NoDup. inversion HwfBs.
+    constructor; auto.
+      eapply filter_wf_block; eauto 1.
+Qed.
+
+Hint Resolve filter_wf_blocks : ssa_filter.
+
+Lemma filter_wf_fdef: forall (HwfF: wf_fdef [M] M f) (HuniqF: uniqFdef f)
+  (Hnouse : fdef_doesnt_use_removed check f),
+  wf_fdef [M'] M' f'.
+Proof.
+  intros. assert (HwfF':=HwfF).
+  assert (G:=filter_preserves_wf_fheader).
+  inv_wf_fdef HwfF'.
+  match goal with
+  | Hentry : getEntryBlock _ = _,
+    HuniqF : uniqFdef _,
+    Hnpred : hasNonePredecessor _ _ = _,
+    HwfBs : wf_blocks _ _ _ _ |- _ =>
+     eapply (@TransCFG.pres_getEntryBlock (Filter check))
+       in Hentry; eauto;
+     eapply (@TransCFG.pres_hasNonePredecessor (Filter check)) 
+       in Hnpred; eauto
+  end.
+  rewrite EQ2 in Hwfb.
+  match goal with
+  | H2: fdef_intro _ _ = _, Hnouse : fdef_doesnt_use_removed check _,
+    H9: wf_blocks _ _ _ _ |- _ =>
+    rewrite H2 in H9;
+    rewrite <- H2 in Hnouse;
+    eapply filter_wf_blocks in H9; try solve [
+      eauto |
+      rewrite <- H2 in HuniqF; eapply uniqF__uniqBlocksLocs; eauto |
+      rewrite <- H2; simpl; intros; apply In_InBlocksB; auto |
+      rewrite <- H2; eapply fdef_doesnt_use_removed_inv; eauto
+    ]
+  end.
+
+  subst. uniq_result.
+  eapply wf_fdef_intro; eauto 2.
+    clear. 
+    apply productInSystemModuleB_intro.
+      simpl. unfold is_true. apply InProductsB_middle.
+
+      unfold moduleInSystem. simpl. apply orb_true_intro. 
+      left. apply moduleEqB_refl.
+Qed.
+
+End WellFormedness.
 
 Lemma filter_wfS: forall check f los nts Ps1 Ps2 
   (HwfS: wf_system [module_intro los nts (Ps1 ++ product_fdef f :: Ps2)])
   (Hunused: fdef_doesnt_use_removed check f),
   wf_system 
     [module_intro los nts (Ps1 ++  product_fdef (filter_fdef check f) :: Ps2)].
-Admitted.
+Proof.
+  intros.
+  assert (HuniqF: uniqFdef f).
+    apply wf_single_system__wf_uniq_fdef in HwfS.
+    destruct HwfS; auto.
+  eapply TopWFS.trans_wfS with (f:=f) in HwfS; intros;
+    eauto using filter_fheader.
+    eapply filter_wf_fdef in HwfF; eauto.
+    eapply filter_fdef__uniqFdef; eauto.
+Qed.
 
-Require Import palloca_props.
+Lemma filter_alloca_in_entry: forall pid pty pnum pal check f
+  (Huniq: uniqFdef f) b
+  (Hisntal: forall c, 
+            lookupInsnViaIDFromFdef f (getCmdLoc c) = ret (insn_cmd c) ->
+            check (insn_cmd c) = false -> 
+            isnt_alloca c) cs
+  (Hex: forall c, In c cs -> cmdInFdefBlockB c f b = true)
+  (H : In (insn_alloca pid pty pnum pal) cs),
+  In (insn_alloca pid pty pnum pal) (filter_cmds check cs).
+Proof.
+  induction cs; simpl; intros; auto.
+    destruct H as [H | H]; subst.
+      destruct_if; simpl; auto.
+        symmetry in HeqR.
+        apply Hisntal in HeqR.
+          inv HeqR.
+
+          match goal with
+          | |- context [getCmdLoc ?c] => 
+               replace (getCmdLoc c) with (getInsnLoc (insn_cmd c)); auto
+          end.
+          apply IngetInsnsLocs__lookupInsnViaIDFromFdef with (b:=b); auto.
+          simpl.
+          apply Hex. auto.
+
+      destruct_if; simpl; auto.
+Qed.
+
+Section FilterPromotable.
+
+Variable (check:insn -> bool) (pid:id).
+
+Lemma filter_used_in_phis: forall ps init
+  (H: fold_left (fun (re : bool) (p : phinode) => re || used_in_phi pid p)
+        ps init = false),
+  fold_left (fun (re : bool) (p : phinode) => re || used_in_phi pid p)
+     (filter_phinodes check ps) init = false.
+Proof.
+  induction ps; simpl; intros; auto.
+    apply fold_left_or_false in H.
+      destruct H as [H1 H2].
+      apply orb_false_iff in H2.
+      destruct H2; subst. 
+      destruct_if; auto.
+        simpl. rewrite H0. auto.
+      
+      apply used_in_phi_fun_spec.
+Qed.
+
+Lemma filter_is_promotable_cmds: forall cs acc
+  (H: fold_left (is_promotable_cmd pid) cs acc = true),
+  fold_left (is_promotable_cmd pid) (filter_cmds check cs) acc =
+    true.
+Proof.
+  induction cs; simpl; intros; auto.
+    apply fold_left_and_true in H.
+      destruct H as [H1 H2].
+      destruct_if.
+        simpl. rewrite H2. auto.
+        apply is_promotable_cmd_spec in H2. subst. auto.
+      apply is_promotable_cmd_spec.
+Qed.
+
+Lemma subst_is_promotable_fun: forall b acc,
+  is_promotable_fun pid acc b = true ->
+  is_promotable_fun pid acc (filter_block check b) = true.
+Proof.
+  destruct b; simpl.
+  intros.
+  match goal with
+  | H: context [if ?lk then _ else _] |- _ =>
+    remember lk as R; destruct R; tinv H
+  end.
+  symmetry in HeqR.
+  assert (forall (a : bool) c, a || c = false -> a = false) as G.
+    intros a c Hin. apply orb_false_iff in Hin. tauto.
+  apply fold_left_or_false in HeqR; eauto 2.
+  destruct HeqR as [J1 J2].
+  apply filter_used_in_phis in J1.
+  rewrite J2. rewrite J1.
+  apply filter_is_promotable_cmds; auto.
+Qed.
+
+Lemma filter_is_promotable_funs: forall bs init
+  (H : fold_left (is_promotable_fun pid) bs init = true),
+  fold_left (is_promotable_fun pid) (List.map (filter_block check) bs) init =
+    true.
+Proof.
+  induction bs; simpl; intros; auto.
+    apply fold_left_and_true in H.
+      destruct H as [H1 H2].
+      rewrite subst_is_promotable_fun; auto.
+      
+      apply is_promotable_fun_spec.
+Qed.
+
+Lemma filter_is_promotable: forall f
+  (H: is_promotable f pid = true),
+  is_promotable (filter_fdef check f) pid = true.
+Proof.
+  unfold is_promotable.
+  destruct f as [fh bs]. simpl. intros.
+  apply filter_is_promotable_funs; auto.
+Qed.
+
+End FilterPromotable.
 
 Lemma filter_wfPI: forall check f los nts Ps1 Ps2 pinfo
   (Hwfpi: WF_PhiInfo pinfo)
@@ -212,59 +1539,34 @@ Lemma filter_wfPI: forall check f los nts Ps1 Ps2 pinfo
             check (insn_cmd c) = false -> 
             isnt_alloca c),
   WF_PhiInfo (update_pinfo pinfo (filter_fdef check f)).
-Admitted.
-
-(*
-Require Import list_facts.
-
-Section uniqueness.
-
-(* Removing an id from an fdef preserves uniqueness *)
-
-Hint Resolve sl_nil sublist_refl.
-
-Lemma remove_block__blockLocs__sublist :
-  forall (id1 : id) (bs : blocks),
-    sublist (getBlocksLocs (List.map (remove_block id1) bs))
-    (getBlocksLocs bs).
 Proof.
-  intros id1 bs. induction bs as [|[lab phis cmds tmn] bs]. apply sl_nil.
-  simpl. repeat apply sublist_app; trivial; clear IHbs.
-  apply sublist_map. apply filter_sublist.
-  induction cmds as [|cmd cmds]. apply sl_nil.
-  simpl. destruct (id_dec (getCmdLoc cmd) id1); simpl;
-  [apply sl_cons_r|apply sl_cons]; trivial.
+  intros. subst.
+  assert (HuniqF: uniqFdef (PI_f pinfo)).
+    apply wf_single_system__wf_uniq_fdef in HwfS; auto.
+    tauto.
+  destruct Hwfpi.
+  destruct pinfo. 
+  split; simpl in *.
+    unfold promotable_alloca in *.
+    inv_mbind. 
+    fold_filter_tac.
+    erewrite TransCFG.pres_getEntryBlock; eauto.
+    destruct b as [l0 ps0 cs0 tmn0]. 
+    destruct H.
+    simpl.
+    split.
+      match goal with
+      | HeqR: ret ?b0 = getEntryBlock _ |- _ =>
+        symmetry in HeqR;
+        apply entryBlockInFdef in HeqR;
+        eapply filter_alloca_in_entry with (b:=b0); eauto 1
+      end.
+      intros. 
+      bsplit; auto.
+        simpl. solve_in_list.
+
+      unfold is_true.
+      apply filter_is_promotable; auto.
+
+    rewrite <- filter_reachablity_analysis; auto.
 Qed.
-
-Lemma remove_block__uniqBlocks :
-  forall (id1 : id) (bs : blocks),
-    uniqBlocks bs -> uniqBlocks (List.map (remove_block id1) bs).
-Proof.
-  intros id1 bs H.
-  split; [destruct H as [H _] | destruct H as [_ H]];
-    apply (NoDup_sublist _ _ _ H); clear H;
-      [|apply remove_block__blockLocs__sublist].
-  induction bs as [|[lab phis cmds tmn] bs]; simpl;
-    [apply sl_nil|apply sl_cons]; trivial.
-Qed.
-
-Lemma remove_fdef__uniqFdef :
-  forall (id1 : id) (f : fdef),
-    uniqFdef f -> uniqFdef (remove_fdef id1 f).
-Proof.
-  intros id1 f H.
-  destruct f as [[att rtyp idf fas fvas] bs].
-  destruct H as [Hbsuniq HNoDup].
-  simpl. split. apply remove_block__uniqBlocks. trivial.
-  apply NoDup_split' in HNoDup. destruct HNoDup as [Hfas [Hbs Hin]].
-  apply NoDup_app. trivial.
-    apply NoDup_sublist with (getBlocksLocs bs). trivial.
-    apply remove_block__blockLocs__sublist.
-
-    intros id' H1 H2. clear Hbsuniq. apply (Hin id' H1).
-    clear H1. generalize id' H2. clear id' H2.
-    apply sublist_In. apply remove_block__blockLocs__sublist.
-Qed.
-
-End uniqueness.
-*)
